Clap/eDSLState/Circuit.lean
@@ -156,7 +156,7 @@ def varsAllocated (c : Circuit) (varStore : VarStore p) (σ : HashConsSt p) (num
   ∀ i (h : i < c.size),
     letI evalSt := [varStore, σ, numAlloc|c.take i]ₑ
     c[i].varsAllocated evalSt.varStore σ ∧
-    ∀ e ∈ c[i].exprs, ∀ x ∈ Expr.varSet ⟨e, σ⟩, x < evalSt.numAlloc
+    ∀ e ∈ c[i].exprs, ⦃e, σ⦄.varSet_wellFormed evalSt.numAlloc
 
 @[simp, grind .]
 lemma varsAllocated_nil : varsAllocated #[] varStore σ numAlloc := by
@@ -349,7 +349,7 @@ lemma varsAllocated_singleton_iff :
     simp at h
     grind
   · unfold varsAllocated
-    grind
+    grind [=Expr.varSet_wellFormed]
 
 end Circuit
 
